

## Study unit 7

### Activity 7-10

Determine  $f \circ f$ ,  $g \circ g$ ,  $g \circ f$ , and  $f \circ g$  in the following cases:

(a)  $f: Z \rightarrow Z$  is defined by the rule  $f(x) = x + 1$  and  $g: Z \rightarrow Z$  is defined by the rule  $g(x) = x - 1$ :

$f \circ f: Z \rightarrow Z$  is defined by  $(f \circ f)(x)$ :

$$\begin{aligned}(f \circ f)(x) &= f(f(x)) \\ &= f(x + 1) \quad (\text{replace } f(x) \text{ by } x + 1) \\ &= (x + 1) + 1 \quad (f(x) = x + 1, \text{ so } f(x + 1) = (x + 1) + 1) \\ &= x + 2.\end{aligned}$$

*Note:* If you want to express what this means in words: if you feed  $f \circ f$  an element  $x$ , it spits out the same thing you get if you feed  $x$  to  $f$  and then feed the result to  $f$  again.

First you feed  $x$  to  $f$  to get  $x + 1$ . Now feeding  $x + 1$  to  $f$  gives you  $(x + 1) + 1 = x + 2$ , because  $f$  takes anything you feed it and adds 1 to it.

$g \circ g: Z \rightarrow Z$  is defined by  $(g \circ g)(x) = g(g(x))$

$$\begin{aligned}&= g(x - 1) \\ &= (x - 1) - 1 \\ &= x - 2.\end{aligned}$$

$g \circ f: Z \rightarrow Z$  is defined by  $(g \circ f)(x) = g(f(x))$

$$\begin{aligned}&= g(x + 1) \quad (\text{replace } f(x) \text{ by } x + 1) \\ &= (x + 1) - 1 \quad (g(x) = x - 1, \text{ so } g(x + 1) = (x + 1) - 1) \\ &= x.\end{aligned}$$

$f \circ g: Z \rightarrow Z$  is defined by  $(f \circ g)(x) = f(g(x))$

$$\begin{aligned}&= f(x - 1) \\ &= (x - 1) + 1 \\ &= x.\end{aligned}$$

(b)  $f: R \rightarrow R$  is defined by  $f(x) = 3x - 2$ , and  
 $g: R \rightarrow R$  is defined by  $g(x) = x^2 + x$ :

$f \circ f: R \rightarrow R$  is defined by  $(f \circ f)(x) = f(f(x))$

$$\begin{aligned}&= f(3x - 2) \quad (\text{replace } f(x) \text{ by } 3x - 2) \\ &= 3(3x - 2) - 2 \quad (f(x) = 3x - 2, \text{ so } f(3x - 2) = 3(3x - 2) - 2) \\ &= 9x - 8.\end{aligned}$$

$g \circ g: \mathbb{R} \rightarrow \mathbb{R}$  is defined by  $(g \circ g)(x) = g(g(x))$

$$\begin{aligned} &= g(x^2 + x) \\ &= (x^2 + x)^2 + (x^2 + x) \\ &= (x^2 + x)(x^2 + x) + (x^2 + x) \\ &= x^4 + 2x^3 + x^2 + x^2 + x \\ &= x^4 + 2x^3 + 2x^2 + x. \end{aligned}$$

$g \circ f: \mathbb{R} \rightarrow \mathbb{R}$  is defined by  $(g \circ f)(x) = g(f(x))$

$$\begin{aligned} &= g(3x - 2) \\ &= (3x - 2)^2 + (3x - 2) \\ &= 9x^2 - 12x + 4 + 3x - 2 \\ &= 9x^2 - 9x + 2. \end{aligned}$$

$f \circ g: \mathbb{R} \rightarrow \mathbb{R}$  is defined by

$$\begin{aligned} (f \circ g)(x) &= f(g(x)) \\ &= f(x^2 + x) \\ &= 3(x^2 + x) - 2 \\ &= 3x^2 + 3x - 2. \end{aligned}$$

(c)  $f: \mathbb{Z}^{\geq} \rightarrow \mathbb{Z}^{\geq}$  is defined by  $f(x) = 113$ , and  
 $g: \mathbb{Z}^{\geq} \rightarrow \mathbb{Z}^{\geq}$  is defined by  $g(x) = x + 1$ :

$$\begin{aligned} f \circ f: \mathbb{Z}^{\geq} \rightarrow \mathbb{Z}^{\geq} \text{ is defined by } (f \circ f)(x) &= f(f(x)) \\ &= f(113) = 113. \end{aligned}$$

$$\begin{aligned} g \circ g: \mathbb{Z}^{\geq} \rightarrow \mathbb{Z}^{\geq} \text{ is defined by } (g \circ g)(x) &= g(g(x)) \\ &= g(x + 1) \\ &= (x + 1) + 1 \\ &= x + 2. \end{aligned}$$

$$\begin{aligned} g \circ f: \mathbb{Z}^{\geq} \rightarrow \mathbb{Z}^{\geq} \text{ is defined by } (g \circ f)(x) &= g(f(x)) \\ &= g(113) \\ &= 113 + 1 \\ &= 114 \end{aligned}$$

$$\begin{aligned} f \circ g: \mathbb{Z}^{\geq} \rightarrow \mathbb{Z}^{\geq} \text{ is defined by } (f \circ g)(x) &= f(g(x)) \\ &= f(x + 1) \\ &= 113. \end{aligned}$$

(because  $f$  does not care what you feed it is constantly going to spit out 113 nothing else).